AuthenticateAction

DynamoDbEncryption/runtimes/java/src/main/smithy-generated/software/amazon/cryptography/dbencryptionsdk/structuredencryption/ToDafny.java
@@ -15,8 +15,6 @@ import java.util.List;
 import java.util.Map;
 import java.util.Objects;
 import software.amazon.cryptography.dbencryptionsdk.structuredencryption.internaldafny.types.AuthenticateAction;
-import software.amazon.cryptography.dbencryptionsdk.structuredencryption.internaldafny.types.AuthenticateSchema;
-import software.amazon.cryptography.dbencryptionsdk.structuredencryption.internaldafny.types.AuthenticateSchemaContent;
 import software.amazon.cryptography.dbencryptionsdk.structuredencryption.internaldafny.types.CryptoAction;
 import software.amazon.cryptography.dbencryptionsdk.structuredencryption.internaldafny.types.DecryptStructureInput;
 import software.amazon.cryptography.dbencryptionsdk.structuredencryption.internaldafny.types.DecryptStructureOutput;
@@ -64,25 +62,14 @@ public class ToDafny {
     return Error.create_CollectionOfErrors(list, message);
   }
 
-  public static AuthenticateSchema AuthenticateSchema(
-      software.amazon.cryptography.dbencryptionsdk.structuredencryption.model.AuthenticateSchema nativeValue) {
-    AuthenticateSchemaContent content;
-    content = ToDafny.AuthenticateSchemaContent(nativeValue.content());
-    Option<DafnyMap<? extends DafnySequence<? extends Character>, ? extends AuthenticateAction>> attributes;
-    attributes = (Objects.nonNull(nativeValue.attributes()) && nativeValue.attributes().size() > 0) ?
-        Option.create_Some(ToDafny.AuthenticateSchemaAttributes(nativeValue.attributes()))
-        : Option.create_None();
-    return new AuthenticateSchema(content, attributes);
-  }
-
   public static DecryptStructureInput DecryptStructureInput(
       software.amazon.cryptography.dbencryptionsdk.structuredencryption.model.DecryptStructureInput nativeValue) {
     DafnySequence<? extends Character> tableName;
     tableName = software.amazon.smithy.dafny.conversion.ToDafny.Simple.CharacterSequence(nativeValue.tableName());
     StructuredData encryptedStructure;
     encryptedStructure = ToDafny.StructuredData(nativeValue.encryptedStructure());
-    AuthenticateSchema authenticateSchema;
-    authenticateSchema = ToDafny.AuthenticateSchema(nativeValue.authenticateSchema());
+    DafnyMap<? extends DafnySequence<? extends Character>, ? extends AuthenticateAction> authenticateSchema;
+    authenticateSchema = ToDafny.AuthenticateSchemaMap(nativeValue.authenticateSchema());
     ICryptographicMaterialsManager cmm;
     cmm = software.amazon.cryptography.materialproviders.ToDafny.CryptographicMaterialsManager(nativeValue.cmm());
     Option<DafnyMap<? extends DafnySequence<? extends Byte>, ? extends DafnySequence<? extends Byte>>> encryptionContext;
@@ -213,20 +200,6 @@ public class ToDafny {
     }
   }
 
-  public static AuthenticateSchemaContent AuthenticateSchemaContent(
-      software.amazon.cryptography.dbencryptionsdk.structuredencryption.model.AuthenticateSchemaContent nativeValue) {
-    if (Objects.nonNull(nativeValue.Action())) {
-      return AuthenticateSchemaContent.create_Action(ToDafny.AuthenticateAction(nativeValue.Action()));
-    }
-    if (Objects.nonNull(nativeValue.SchemaMap())) {
-      return AuthenticateSchemaContent.create_SchemaMap(ToDafny.AuthenticateSchemaMap(nativeValue.SchemaMap()));
-    }
-    if (Objects.nonNull(nativeValue.SchemaList())) {
-      return AuthenticateSchemaContent.create_SchemaList(ToDafny.AuthenticateSchemaList(nativeValue.SchemaList()));
-    }
-    throw new IllegalArgumentException("Cannot convert " + nativeValue + " to software.amazon.cryptography.dbencryptionsdk.structuredencryption.internaldafny.types.AuthenticateSchemaContent.");
-  }
-
   public static StructuredDataContent StructuredDataContent(
       software.amazon.cryptography.dbencryptionsdk.structuredencryption.model.StructuredDataContent nativeValue) {
     if (Objects.nonNull(nativeValue.Terminal())) {
@@ -241,14 +214,6 @@ public class ToDafny {
     throw new IllegalArgumentException("Cannot convert " + nativeValue + " to software.amazon.cryptography.dbencryptionsdk.structuredencryption.internaldafny.types.StructuredDataContent.");
   }
 
-  public static DafnySequence<? extends AuthenticateSchema> AuthenticateSchemaList(
-      List<software.amazon.cryptography.dbencryptionsdk.structuredencryption.model.AuthenticateSchema> nativeValue) {
-    return software.amazon.smithy.dafny.conversion.ToDafny.Aggregate.GenericToSequence(
-        nativeValue, 
-        software.amazon.cryptography.dbencryptionsdk.structuredencryption.ToDafny::AuthenticateSchema, 
-        AuthenticateSchema._typeDescriptor());
-  }
-
   public static DafnySequence<? extends StructuredData> StructuredDataList(
       List<software.amazon.cryptography.dbencryptionsdk.structuredencryption.model.StructuredData> nativeValue) {
     return software.amazon.smithy.dafny.conversion.ToDafny.Aggregate.GenericToSequence(
@@ -257,20 +222,12 @@ public class ToDafny {
         StructuredData._typeDescriptor());
   }
 
-  public static DafnyMap<? extends DafnySequence<? extends Character>, ? extends AuthenticateAction> AuthenticateSchemaAttributes(
+  public static DafnyMap<? extends DafnySequence<? extends Character>, ? extends AuthenticateAction> AuthenticateSchemaMap(
       Map<String, software.amazon.cryptography.dbencryptionsdk.structuredencryption.model.AuthenticateAction> nativeValue) {
     return software.amazon.smithy.dafny.conversion.ToDafny.Aggregate.GenericToMap(
         nativeValue, 
         software.amazon.smithy.dafny.conversion.ToDafny.Simple::CharacterSequence, 
         software.amazon.cryptography.dbencryptionsdk.structuredencryption.ToDafny::AuthenticateAction);
-  }
-
-  public static DafnyMap<? extends DafnySequence<? extends Character>, ? extends AuthenticateSchema> AuthenticateSchemaMap(
-      Map<String, software.amazon.cryptography.dbencryptionsdk.structuredencryption.model.AuthenticateSchema> nativeValue) {
-    return software.amazon.smithy.dafny.conversion.ToDafny.Aggregate.GenericToMap(
-        nativeValue, 
-        software.amazon.smithy.dafny.conversion.ToDafny.Simple::CharacterSequence, 
-        software.amazon.cryptography.dbencryptionsdk.structuredencryption.ToDafny::AuthenticateSchema);
   }
 
   public static DafnyMap<? extends DafnySequence<? extends Character>, ? extends CryptoAction> CryptoSchemaMap(
