DynamoDbEncryption/runtimes/net/Generated/DynamoDbEncryption/TypeConversion.cs
@@ -1357,10 +1357,6 @@ namespace AWS.Cryptography.DbEncryptionSDK.DynamoDb
     {
       switch (value)
       {
-        case software.amazon.cryptography.dbencryptionsdk.dynamodb.internaldafny.types.Error_AwsCryptographyPrimitives dafnyVal:
-          return AWS.Cryptography.Primitives.TypeConversion.FromDafny_CommonError(
-            dafnyVal._AwsCryptographyPrimitives
-          );
         case software.amazon.cryptography.dbencryptionsdk.dynamodb.internaldafny.types.Error_AwsCryptographyDbEncryptionSdkStructuredEncryption dafnyVal:
           return AWS.Cryptography.DbEncryptionSDK.StructuredEncryption.TypeConversion.FromDafny_CommonError(
             dafnyVal._AwsCryptographyDbEncryptionSdkStructuredEncryption
@@ -1368,6 +1364,10 @@ namespace AWS.Cryptography.DbEncryptionSDK.DynamoDb
         case software.amazon.cryptography.dbencryptionsdk.dynamodb.internaldafny.types.Error_ComAmazonawsDynamodb dafnyVal:
           return Com.Amazonaws.Dynamodb.TypeConversion.FromDafny_CommonError(
             dafnyVal._ComAmazonawsDynamodb
+          );
+        case software.amazon.cryptography.dbencryptionsdk.dynamodb.internaldafny.types.Error_AwsCryptographyPrimitives dafnyVal:
+          return AWS.Cryptography.Primitives.TypeConversion.FromDafny_CommonError(
+            dafnyVal._AwsCryptographyPrimitives
           );
         case software.amazon.cryptography.dbencryptionsdk.dynamodb.internaldafny.types.Error_AwsCryptographyMaterialProviders dafnyVal:
           return AWS.Cryptography.MaterialProviders.TypeConversion.FromDafny_CommonError(
