DynamoDbEncryption/runtimes/net/Generated/DynamoDbEncryptionTransforms/TypeConversion.cs
@@ -6493,6 +6493,10 @@ namespace AWS.Cryptography.DbEncryptionSDK.DynamoDb.Transforms
           return AWS.Cryptography.DbEncryptionSDK.StructuredEncryption.TypeConversion.FromDafny_CommonError(
             dafnyVal._AwsCryptographyDbEncryptionSdkStructuredEncryption
           );
+        case software.amazon.cryptography.dbencryptionsdk.dynamodb.transforms.internaldafny.types.Error_ComAmazonawsDynamodb dafnyVal:
+          return Com.Amazonaws.Dynamodb.TypeConversion.FromDafny_CommonError(
+            dafnyVal._ComAmazonawsDynamodb
+          );
         case software.amazon.cryptography.dbencryptionsdk.dynamodb.transforms.internaldafny.types.Error_AwsCryptographyDbEncryptionSdkDynamoDb dafnyVal:
           return AWS.Cryptography.DbEncryptionSDK.DynamoDb.TypeConversion.FromDafny_CommonError(
             dafnyVal._AwsCryptographyDbEncryptionSdkDynamoDb
@@ -6500,10 +6504,6 @@ namespace AWS.Cryptography.DbEncryptionSDK.DynamoDb.Transforms
         case software.amazon.cryptography.dbencryptionsdk.dynamodb.transforms.internaldafny.types.Error_AwsCryptographyMaterialProviders dafnyVal:
           return AWS.Cryptography.MaterialProviders.TypeConversion.FromDafny_CommonError(
             dafnyVal._AwsCryptographyMaterialProviders
-          );
-        case software.amazon.cryptography.dbencryptionsdk.dynamodb.transforms.internaldafny.types.Error_ComAmazonawsDynamodb dafnyVal:
-          return Com.Amazonaws.Dynamodb.TypeConversion.FromDafny_CommonError(
-            dafnyVal._ComAmazonawsDynamodb
           );
         case software.amazon.cryptography.dbencryptionsdk.dynamodb.transforms.internaldafny.types.Error_DynamoDbEncryptionTransformsException dafnyVal:
           return FromDafny_N3_aws__N12_cryptography__N15_dbEncryptionSdk__N8_dynamoDb__N10_transforms__S37_DynamoDbEncryptionTransformsException(dafnyVal);
