DynamoDbEncryption/dafny/StructuredEncryption/Model/AwsCryptographyDbEncryptionSdkStructuredEncryptionTypes.dfy
@@ -2,336 +2,326 @@
 // SPDX-License-Identifier: Apache-2.0
 // Do not modify this file. This file is machine generated, and any changes to it will be overwritten.
 include "../../../../submodules/MaterialProviders/StandardLibrary/src/Index.dfy"
- include "../../../../submodules/MaterialProviders/AwsCryptographicMaterialProviders/dafny/AwsCryptographicMaterialProviders/src/Index.dfy"
- include "../../../../submodules/MaterialProviders/AwsCryptographyPrimitives/src/Index.dfy"
- module {:extern "software.amazon.cryptography.dbencryptionsdk.structuredencryption.internaldafny.types" } AwsCryptographyDbEncryptionSdkStructuredEncryptionTypes
- {
- import opened Wrappers
- import opened StandardLibrary.UInt
- import opened UTF8
- import AwsCryptographyMaterialProvidersTypes
- import AwsCryptographyPrimitivesTypes
- // Generic helpers for verification of mock/unit tests.
- datatype DafnyCallEvent<I, O> = DafnyCallEvent(input: I, output: O)
- 
- // Begin Generated Types
- 
- datatype AuthenticateAction =
-	| SIGN
-	| DO_NOT_SIGN
- datatype AuthenticateSchema = | AuthenticateSchema (
- nameonly content: AuthenticateSchemaContent ,
- nameonly attributes: Option<AuthenticateSchemaAttributes> := Option.None
- )
- type AuthenticateSchemaAttributes = map<string, AuthenticateAction>
- datatype AuthenticateSchemaContent =
- | Action(Action: AuthenticateAction)
- | SchemaMap(SchemaMap: AuthenticateSchemaMap)
- | SchemaList(SchemaList: AuthenticateSchemaList)
- type AuthenticateSchemaList = seq<AuthenticateSchema>
- type AuthenticateSchemaMap = map<string, AuthenticateSchema>
- datatype CryptoAction =
-	| ENCRYPT_AND_SIGN
-	| SIGN_AND_INCLUDE_IN_ENCRYPTION_CONTEXT
-	| SIGN_ONLY
-	| DO_NOTHING
- type CryptoSchemaMap = map<string, CryptoAction>
- datatype DecryptStructureInput = | DecryptStructureInput (
- nameonly tableName: string ,
- nameonly encryptedStructure: StructuredData ,
- nameonly authenticateSchema: AuthenticateSchema ,
- nameonly cmm: AwsCryptographyMaterialProvidersTypes.ICryptographicMaterialsManager ,
- nameonly encryptionContext: Option<AwsCryptographyMaterialProvidersTypes.EncryptionContext> := Option.None
- )
- datatype DecryptStructureOutput = | DecryptStructureOutput (
- nameonly plaintextStructure: StructuredData ,
- nameonly parsedHeader: ParsedHeader
- )
- datatype EncryptStructureInput = | EncryptStructureInput (
- nameonly tableName: string ,
- nameonly plaintextStructure: StructuredData ,
- nameonly cryptoSchema: CryptoSchemaMap ,
- nameonly cmm: AwsCryptographyMaterialProvidersTypes.ICryptographicMaterialsManager ,
- nameonly algorithmSuiteId: Option<AwsCryptographyMaterialProvidersTypes.DBEAlgorithmSuiteId> := Option.None ,
- nameonly encryptionContext: Option<AwsCryptographyMaterialProvidersTypes.EncryptionContext> := Option.None
- )
- datatype EncryptStructureOutput = | EncryptStructureOutput (
- nameonly encryptedStructure: StructuredData ,
- nameonly parsedHeader: ParsedHeader
- )
- datatype ParsedHeader = | ParsedHeader (
- nameonly cryptoSchema: CryptoSchemaMap ,
- nameonly algorithmSuiteId: AwsCryptographyMaterialProvidersTypes.DBEAlgorithmSuiteId ,
- nameonly encryptedDataKeys: AwsCryptographyMaterialProvidersTypes.EncryptedDataKeyList ,
- nameonly storedEncryptionContext: AwsCryptographyMaterialProvidersTypes.EncryptionContext ,
- nameonly encryptionContext: AwsCryptographyMaterialProvidersTypes.EncryptionContext
- )
- datatype StructuredData = | StructuredData (
- nameonly content: StructuredDataContent ,
- nameonly attributes: Option<StructuredDataAttributes> := Option.None
- )
- type StructuredDataAttributes = map<string, StructuredDataTerminal>
- datatype StructuredDataContent =
- | Terminal(Terminal: StructuredDataTerminal)
- | DataList(DataList: StructuredDataList)
- | DataMap(DataMap: StructuredDataMap)
- type StructuredDataList = seq<StructuredData>
- type StructuredDataMap = map<string, StructuredData>
- datatype StructuredDataTerminal = | StructuredDataTerminal (
- nameonly value: TerminalValue ,
- nameonly typeId: TerminalTypeId
- )
- class IStructuredEncryptionClientCallHistory {
- ghost constructor() {
- EncryptStructure := [];
- DecryptStructure := [];
-}
- ghost var EncryptStructure: seq<DafnyCallEvent<EncryptStructureInput, Result<EncryptStructureOutput, Error>>>
- ghost var DecryptStructure: seq<DafnyCallEvent<DecryptStructureInput, Result<DecryptStructureOutput, Error>>>
-}
- trait {:termination false} IStructuredEncryptionClient
- {
- // Helper to define any additional modifies/reads clauses.
- // If your operations need to mutate state,
- // add it in your constructor function:
- // Modifies := {your, fields, here, History};
- // If you do not need to mutate anything:
-// Modifies := {History};
+include "../../../../submodules/MaterialProviders/AwsCryptographicMaterialProviders/dafny/AwsCryptographicMaterialProviders/src/Index.dfy"
+include "../../../../submodules/MaterialProviders/AwsCryptographyPrimitives/src/Index.dfy"
+module {:extern "software.amazon.cryptography.dbencryptionsdk.structuredencryption.internaldafny.types" } AwsCryptographyDbEncryptionSdkStructuredEncryptionTypes
+{
+  import opened Wrappers
+  import opened StandardLibrary.UInt
+  import opened UTF8
+  import AwsCryptographyMaterialProvidersTypes
+  import AwsCryptographyPrimitivesTypes
+    // Generic helpers for verification of mock/unit tests.
+  datatype DafnyCallEvent<I, O> = DafnyCallEvent(input: I, output: O)
 
- ghost const Modifies: set<object>
- // For an unassigned field defined in a trait,
- // Dafny can only assign a value in the constructor.
- // This means that for Dafny to reason about this value,
- // it needs some way to know (an invariant),
- // about the state of the object.
- // This builds on the Valid/Repr paradigm
- // To make this kind requires safe to add
- // to methods called from unverified code,
- // the predicate MUST NOT take any arguments.
- // This means that the correctness of this requires
- // MUST only be evaluated by the class itself.
- // If you require any additional mutation,
- // then you MUST ensure everything you need in ValidState.
- // You MUST also ensure ValidState in your constructor.
- predicate ValidState()
- ensures ValidState() ==> History in Modifies
-  ghost const History: IStructuredEncryptionClientCallHistory
- predicate EncryptStructureEnsuresPublicly(input: EncryptStructureInput , output: Result<EncryptStructureOutput, Error>)
- // The public method to be called by library consumers
- method EncryptStructure ( input: EncryptStructureInput )
- returns (output: Result<EncryptStructureOutput, Error>)
- requires
- && ValidState()
- && input.cmm.ValidState()
- && input.cmm.Modifies !! {History}
- modifies Modifies - {History} ,
- input.cmm.Modifies ,
- History`EncryptStructure
- // Dafny will skip type parameters when generating a default decreases clause.
- decreases Modifies - {History} ,
- input.cmm.Modifies
- ensures
- && ValidState()
- ensures EncryptStructureEnsuresPublicly(input, output)
- ensures History.EncryptStructure == old(History.EncryptStructure) + [DafnyCallEvent(input, output)]
- 
- predicate DecryptStructureEnsuresPublicly(input: DecryptStructureInput , output: Result<DecryptStructureOutput, Error>)
- // The public method to be called by library consumers
- method DecryptStructure ( input: DecryptStructureInput )
- returns (output: Result<DecryptStructureOutput, Error>)
- requires
- && ValidState()
- && input.cmm.ValidState()
- && input.cmm.Modifies !! {History}
- modifies Modifies - {History} ,
- input.cmm.Modifies ,
- History`DecryptStructure
- // Dafny will skip type parameters when generating a default decreases clause.
- decreases Modifies - {History} ,
- input.cmm.Modifies
- ensures
- && ValidState()
- ensures DecryptStructureEnsuresPublicly(input, output)
- ensures History.DecryptStructure == old(History.DecryptStructure) + [DafnyCallEvent(input, output)]
- 
-}
- datatype StructuredEncryptionConfig = | StructuredEncryptionConfig (
- 
- )
- type TerminalTypeId = x: seq<uint8> | IsValid_TerminalTypeId(x) witness *
- predicate method IsValid_TerminalTypeId(x: seq<uint8>) {
- ( 2 <= |x| <= 2 )
-}
- type TerminalValue = seq<uint8>
- type Version = x: int32 | IsValid_Version(x) witness *
- predicate method IsValid_Version(x: int32) {
- ( 1 <= x <= 1 )
-}
- datatype Error =
- // Local Error structures are listed here
- | StructuredEncryptionException (
- nameonly message: string
- )
- // Any dependent models are listed here
- | AwsCryptographyMaterialProviders(AwsCryptographyMaterialProviders: AwsCryptographyMaterialProvidersTypes.Error)
- | AwsCryptographyPrimitives(AwsCryptographyPrimitives: AwsCryptographyPrimitivesTypes.Error)
- // The Collection error is used to collect several errors together
- // This is useful when composing OR logic.
- // Consider the following method:
- // 
- // method FN<I, O>(n:I)
- //   returns (res: Result<O, Types.Error>)
- //   ensures A(I).Success? ==> res.Success?
- //   ensures B(I).Success? ==> res.Success?
- //   ensures A(I).Failure? && B(I).Failure? ==> res.Failure?
- // 
- // If either A || B is successful then FN is successful.
- // And if A && B fail then FN will fail.
- // But what information should FN transmit back to the caller?
- // While it may be correct to hide these details from the caller,
- // this can not be the globally correct option.
- // Suppose that A and B can be blocked by different ACLs,
- // and that their representation of I is only eventually consistent.
- // How can the caller distinguish, at a minimum for logging,
- // the difference between the four failure modes?
- // || (!access(A(I)) && !access(B(I)))
- // || (!exit(A(I)) && !exit(B(I)))
- // || (!access(A(I)) && !exit(B(I)))
- // || (!exit(A(I)) && !access(B(I)))
- | CollectionOfErrors(list: seq<Error>, nameonly message: string)
- // The Opaque error, used for native, extern, wrapped or unknown errors
- | Opaque(obj: object)
- type OpaqueError = e: Error | e.Opaque? witness *
-}
- abstract module AbstractAwsCryptographyDbEncryptionSdkStructuredEncryptionService
- {
- import opened Wrappers
- import opened StandardLibrary.UInt
- import opened UTF8
- import opened Types = AwsCryptographyDbEncryptionSdkStructuredEncryptionTypes
- import Operations : AbstractAwsCryptographyDbEncryptionSdkStructuredEncryptionOperations
- function method DefaultStructuredEncryptionConfig(): StructuredEncryptionConfig
- method StructuredEncryption(config: StructuredEncryptionConfig := DefaultStructuredEncryptionConfig())
- returns (res: Result<IStructuredEncryptionClient, Error>)
- ensures res.Success? ==> 
- && fresh(res.value)
- && fresh(res.value.Modifies)
- && fresh(res.value.History)
- && res.value.ValidState()
+  // Begin Generated Types
 
- // Helper function for the benefit of native code to create a Success(client) without referring to Dafny internals
- function method CreateSuccessOfClient(client: IStructuredEncryptionClient): Result<IStructuredEncryptionClient, Error> {
-   Success(client)
- } // Helper function for the benefit of native code to create a Failure(error) without referring to Dafny internals
- function method CreateFailureOfError(error: Error): Result<IStructuredEncryptionClient, Error> {
-   Failure(error)
- }
- class StructuredEncryptionClient extends IStructuredEncryptionClient
- {
- constructor(config: Operations.InternalConfig)
- requires Operations.ValidInternalConfig?(config)
- ensures
- && ValidState()
- && fresh(History)
- && this.config == config
- const config: Operations.InternalConfig
- predicate ValidState()
- ensures ValidState() ==>
- && Operations.ValidInternalConfig?(config)
- && History !in Operations.ModifiesInternalConfig(config)
- && Modifies == Operations.ModifiesInternalConfig(config) + {History}
- predicate EncryptStructureEnsuresPublicly(input: EncryptStructureInput , output: Result<EncryptStructureOutput, Error>)
- {Operations.EncryptStructureEnsuresPublicly(input, output)}
- // The public method to be called by library consumers
- method EncryptStructure ( input: EncryptStructureInput )
- returns (output: Result<EncryptStructureOutput, Error>)
- requires
- && ValidState()
- && input.cmm.ValidState()
- && input.cmm.Modifies !! {History}
- modifies Modifies - {History} ,
- input.cmm.Modifies ,
- History`EncryptStructure
- // Dafny will skip type parameters when generating a default decreases clause.
- decreases Modifies - {History} ,
- input.cmm.Modifies
- ensures
- && ValidState()
- ensures EncryptStructureEnsuresPublicly(input, output)
- ensures History.EncryptStructure == old(History.EncryptStructure) + [DafnyCallEvent(input, output)]
- {
- output := Operations.EncryptStructure(config, input);
- History.EncryptStructure := History.EncryptStructure + [DafnyCallEvent(input, output)];
+  datatype AuthenticateAction =
+    | SIGN
+    | DO_NOT_SIGN
+  type AuthenticateSchemaMap = map<string, AuthenticateAction>
+  datatype CryptoAction =
+    | ENCRYPT_AND_SIGN
+    | SIGN_AND_INCLUDE_IN_ENCRYPTION_CONTEXT
+    | SIGN_ONLY
+    | DO_NOTHING
+  type CryptoSchemaMap = map<string, CryptoAction>
+  datatype DecryptStructureInput = | DecryptStructureInput (
+    nameonly tableName: string ,
+    nameonly encryptedStructure: StructuredData ,
+    nameonly authenticateSchema: AuthenticateSchemaMap ,
+    nameonly cmm: AwsCryptographyMaterialProvidersTypes.ICryptographicMaterialsManager ,
+    nameonly encryptionContext: Option<AwsCryptographyMaterialProvidersTypes.EncryptionContext> := Option.None
+  )
+  datatype DecryptStructureOutput = | DecryptStructureOutput (
+    nameonly plaintextStructure: StructuredData ,
+    nameonly parsedHeader: ParsedHeader
+  )
+  datatype EncryptStructureInput = | EncryptStructureInput (
+    nameonly tableName: string ,
+    nameonly plaintextStructure: StructuredData ,
+    nameonly cryptoSchema: CryptoSchemaMap ,
+    nameonly cmm: AwsCryptographyMaterialProvidersTypes.ICryptographicMaterialsManager ,
+    nameonly algorithmSuiteId: Option<AwsCryptographyMaterialProvidersTypes.DBEAlgorithmSuiteId> := Option.None ,
+    nameonly encryptionContext: Option<AwsCryptographyMaterialProvidersTypes.EncryptionContext> := Option.None
+  )
+  datatype EncryptStructureOutput = | EncryptStructureOutput (
+    nameonly encryptedStructure: StructuredData ,
+    nameonly parsedHeader: ParsedHeader
+  )
+  datatype ParsedHeader = | ParsedHeader (
+    nameonly cryptoSchema: CryptoSchemaMap ,
+    nameonly algorithmSuiteId: AwsCryptographyMaterialProvidersTypes.DBEAlgorithmSuiteId ,
+    nameonly encryptedDataKeys: AwsCryptographyMaterialProvidersTypes.EncryptedDataKeyList ,
+    nameonly storedEncryptionContext: AwsCryptographyMaterialProvidersTypes.EncryptionContext ,
+    nameonly encryptionContext: AwsCryptographyMaterialProvidersTypes.EncryptionContext
+  )
+  datatype StructuredData = | StructuredData (
+    nameonly content: StructuredDataContent ,
+    nameonly attributes: Option<StructuredDataAttributes> := Option.None
+  )
+  type StructuredDataAttributes = map<string, StructuredDataTerminal>
+  datatype StructuredDataContent =
+    | Terminal(Terminal: StructuredDataTerminal)
+    | DataList(DataList: StructuredDataList)
+    | DataMap(DataMap: StructuredDataMap)
+  type StructuredDataList = seq<StructuredData>
+  type StructuredDataMap = map<string, StructuredData>
+  datatype StructuredDataTerminal = | StructuredDataTerminal (
+    nameonly value: TerminalValue ,
+    nameonly typeId: TerminalTypeId
+  )
+  class IStructuredEncryptionClientCallHistory {
+    ghost constructor() {
+      EncryptStructure := [];
+      DecryptStructure := [];
+    }
+    ghost var EncryptStructure: seq<DafnyCallEvent<EncryptStructureInput, Result<EncryptStructureOutput, Error>>>
+    ghost var DecryptStructure: seq<DafnyCallEvent<DecryptStructureInput, Result<DecryptStructureOutput, Error>>>
+  }
+  trait {:termination false} IStructuredEncryptionClient
+  {
+    // Helper to define any additional modifies/reads clauses.
+    // If your operations need to mutate state,
+    // add it in your constructor function:
+    // Modifies := {your, fields, here, History};
+    // If you do not need to mutate anything:
+    // Modifies := {History};
+
+    ghost const Modifies: set<object>
+    // For an unassigned field defined in a trait,
+    // Dafny can only assign a value in the constructor.
+    // This means that for Dafny to reason about this value,
+    // it needs some way to know (an invariant),
+    // about the state of the object.
+    // This builds on the Valid/Repr paradigm
+    // To make this kind requires safe to add
+    // to methods called from unverified code,
+    // the predicate MUST NOT take any arguments.
+    // This means that the correctness of this requires
+    // MUST only be evaluated by the class itself.
+    // If you require any additional mutation,
+    // then you MUST ensure everything you need in ValidState.
+    // You MUST also ensure ValidState in your constructor.
+    predicate ValidState()
+      ensures ValidState() ==> History in Modifies
+    ghost const History: IStructuredEncryptionClientCallHistory
+    predicate EncryptStructureEnsuresPublicly(input: EncryptStructureInput , output: Result<EncryptStructureOutput, Error>)
+    // The public method to be called by library consumers
+    method EncryptStructure ( input: EncryptStructureInput )
+      returns (output: Result<EncryptStructureOutput, Error>)
+      requires
+        && ValidState()
+        && input.cmm.ValidState()
+        && input.cmm.Modifies !! {History}
+      modifies Modifies - {History} ,
+               input.cmm.Modifies ,
+               History`EncryptStructure
+      // Dafny will skip type parameters when generating a default decreases clause.
+      decreases Modifies - {History} ,
+                input.cmm.Modifies
+      ensures
+        && ValidState()
+      ensures EncryptStructureEnsuresPublicly(input, output)
+      ensures History.EncryptStructure == old(History.EncryptStructure) + [DafnyCallEvent(input, output)]
+
+    predicate DecryptStructureEnsuresPublicly(input: DecryptStructureInput , output: Result<DecryptStructureOutput, Error>)
+    // The public method to be called by library consumers
+    method DecryptStructure ( input: DecryptStructureInput )
+      returns (output: Result<DecryptStructureOutput, Error>)
+      requires
+        && ValidState()
+        && input.cmm.ValidState()
+        && input.cmm.Modifies !! {History}
+      modifies Modifies - {History} ,
+               input.cmm.Modifies ,
+               History`DecryptStructure
+      // Dafny will skip type parameters when generating a default decreases clause.
+      decreases Modifies - {History} ,
+                input.cmm.Modifies
+      ensures
+        && ValidState()
+      ensures DecryptStructureEnsuresPublicly(input, output)
+      ensures History.DecryptStructure == old(History.DecryptStructure) + [DafnyCallEvent(input, output)]
+
+  }
+  datatype StructuredEncryptionConfig = | StructuredEncryptionConfig (
+
+                                        )
+  type TerminalTypeId = x: seq<uint8> | IsValid_TerminalTypeId(x) witness *
+  predicate method IsValid_TerminalTypeId(x: seq<uint8>) {
+    ( 2 <= |x| <= 2 )
+  }
+  type TerminalValue = seq<uint8>
+  type Version = x: int32 | IsValid_Version(x) witness *
+  predicate method IsValid_Version(x: int32) {
+    ( 1 <= x <= 1 )
+  }
+  datatype Error =
+      // Local Error structures are listed here
+    | StructuredEncryptionException (
+        nameonly message: string
+      )
+      // Any dependent models are listed here
+    | AwsCryptographyMaterialProviders(AwsCryptographyMaterialProviders: AwsCryptographyMaterialProvidersTypes.Error)
+    | AwsCryptographyPrimitives(AwsCryptographyPrimitives: AwsCryptographyPrimitivesTypes.Error)
+      // The Collection error is used to collect several errors together
+      // This is useful when composing OR logic.
+      // Consider the following method:
+      // 
+      // method FN<I, O>(n:I)
+      //   returns (res: Result<O, Types.Error>)
+      //   ensures A(I).Success? ==> res.Success?
+      //   ensures B(I).Success? ==> res.Success?
+      //   ensures A(I).Failure? && B(I).Failure? ==> res.Failure?
+      // 
+      // If either A || B is successful then FN is successful.
+      // And if A && B fail then FN will fail.
+      // But what information should FN transmit back to the caller?
+      // While it may be correct to hide these details from the caller,
+      // this can not be the globally correct option.
+      // Suppose that A and B can be blocked by different ACLs,
+      // and that their representation of I is only eventually consistent.
+      // How can the caller distinguish, at a minimum for logging,
+      // the difference between the four failure modes?
+    // || (!access(A(I)) && !access(B(I)))
+    // || (!exit(A(I)) && !exit(B(I)))
+    // || (!access(A(I)) && !exit(B(I)))
+    // || (!exit(A(I)) && !access(B(I)))
+    | CollectionOfErrors(list: seq<Error>, nameonly message: string)
+      // The Opaque error, used for native, extern, wrapped or unknown errors
+    | Opaque(obj: object)
+  type OpaqueError = e: Error | e.Opaque? witness *
 }
- 
- predicate DecryptStructureEnsuresPublicly(input: DecryptStructureInput , output: Result<DecryptStructureOutput, Error>)
- {Operations.DecryptStructureEnsuresPublicly(input, output)}
- // The public method to be called by library consumers
- method DecryptStructure ( input: DecryptStructureInput )
- returns (output: Result<DecryptStructureOutput, Error>)
- requires
- && ValidState()
- && input.cmm.ValidState()
- && input.cmm.Modifies !! {History}
- modifies Modifies - {History} ,
- input.cmm.Modifies ,
- History`DecryptStructure
- // Dafny will skip type parameters when generating a default decreases clause.
- decreases Modifies - {History} ,
- input.cmm.Modifies
- ensures
- && ValidState()
- ensures DecryptStructureEnsuresPublicly(input, output)
- ensures History.DecryptStructure == old(History.DecryptStructure) + [DafnyCallEvent(input, output)]
- {
- output := Operations.DecryptStructure(config, input);
- History.DecryptStructure := History.DecryptStructure + [DafnyCallEvent(input, output)];
+abstract module AbstractAwsCryptographyDbEncryptionSdkStructuredEncryptionService
+{
+  import opened Wrappers
+  import opened StandardLibrary.UInt
+  import opened UTF8
+  import opened Types = AwsCryptographyDbEncryptionSdkStructuredEncryptionTypes
+  import Operations : AbstractAwsCryptographyDbEncryptionSdkStructuredEncryptionOperations
+  function method DefaultStructuredEncryptionConfig(): StructuredEncryptionConfig
+  method StructuredEncryption(config: StructuredEncryptionConfig := DefaultStructuredEncryptionConfig())
+    returns (res: Result<IStructuredEncryptionClient, Error>)
+    ensures res.Success? ==>
+              && fresh(res.value)
+              && fresh(res.value.Modifies)
+              && fresh(res.value.History)
+              && res.value.ValidState()
+
+  // Helper function for the benefit of native code to create a Success(client) without referring to Dafny internals
+  function method CreateSuccessOfClient(client: IStructuredEncryptionClient): Result<IStructuredEncryptionClient, Error> {
+    Success(client)
+  } // Helper function for the benefit of native code to create a Failure(error) without referring to Dafny internals
+  function method CreateFailureOfError(error: Error): Result<IStructuredEncryptionClient, Error> {
+    Failure(error)
+  }
+  class StructuredEncryptionClient extends IStructuredEncryptionClient
+  {
+    constructor(config: Operations.InternalConfig)
+      requires Operations.ValidInternalConfig?(config)
+      ensures
+        && ValidState()
+        && fresh(History)
+        && this.config == config
+    const config: Operations.InternalConfig
+    predicate ValidState()
+      ensures ValidState() ==>
+                && Operations.ValidInternalConfig?(config)
+                && History !in Operations.ModifiesInternalConfig(config)
+                && Modifies == Operations.ModifiesInternalConfig(config) + {History}
+    predicate EncryptStructureEnsuresPublicly(input: EncryptStructureInput , output: Result<EncryptStructureOutput, Error>)
+    {Operations.EncryptStructureEnsuresPublicly(input, output)}
+    // The public method to be called by library consumers
+    method EncryptStructure ( input: EncryptStructureInput )
+      returns (output: Result<EncryptStructureOutput, Error>)
+      requires
+        && ValidState()
+        && input.cmm.ValidState()
+        && input.cmm.Modifies !! {History}
+      modifies Modifies - {History} ,
+               input.cmm.Modifies ,
+               History`EncryptStructure
+      // Dafny will skip type parameters when generating a default decreases clause.
+      decreases Modifies - {History} ,
+                input.cmm.Modifies
+      ensures
+        && ValidState()
+      ensures EncryptStructureEnsuresPublicly(input, output)
+      ensures History.EncryptStructure == old(History.EncryptStructure) + [DafnyCallEvent(input, output)]
+    {
+      output := Operations.EncryptStructure(config, input);
+      History.EncryptStructure := History.EncryptStructure + [DafnyCallEvent(input, output)];
+    }
+
+    predicate DecryptStructureEnsuresPublicly(input: DecryptStructureInput , output: Result<DecryptStructureOutput, Error>)
+    {Operations.DecryptStructureEnsuresPublicly(input, output)}
+    // The public method to be called by library consumers
+    method DecryptStructure ( input: DecryptStructureInput )
+      returns (output: Result<DecryptStructureOutput, Error>)
+      requires
+        && ValidState()
+        && input.cmm.ValidState()
+        && input.cmm.Modifies !! {History}
+      modifies Modifies - {History} ,
+               input.cmm.Modifies ,
+               History`DecryptStructure
+      // Dafny will skip type parameters when generating a default decreases clause.
+      decreases Modifies - {History} ,
+                input.cmm.Modifies
+      ensures
+        && ValidState()
+      ensures DecryptStructureEnsuresPublicly(input, output)
+      ensures History.DecryptStructure == old(History.DecryptStructure) + [DafnyCallEvent(input, output)]
+    {
+      output := Operations.DecryptStructure(config, input);
+      History.DecryptStructure := History.DecryptStructure + [DafnyCallEvent(input, output)];
+    }
+
+  }
 }
- 
-}
-}
- abstract module AbstractAwsCryptographyDbEncryptionSdkStructuredEncryptionOperations {
- import opened Wrappers
- import opened StandardLibrary.UInt
- import opened UTF8
- import opened Types = AwsCryptographyDbEncryptionSdkStructuredEncryptionTypes
- type InternalConfig
- predicate ValidInternalConfig?(config: InternalConfig)
- function ModifiesInternalConfig(config: InternalConfig): set<object>
- predicate EncryptStructureEnsuresPublicly(input: EncryptStructureInput , output: Result<EncryptStructureOutput, Error>)
- // The private method to be refined by the library developer
+abstract module AbstractAwsCryptographyDbEncryptionSdkStructuredEncryptionOperations {
+  import opened Wrappers
+  import opened StandardLibrary.UInt
+  import opened UTF8
+  import opened Types = AwsCryptographyDbEncryptionSdkStructuredEncryptionTypes
+  type InternalConfig
+  predicate ValidInternalConfig?(config: InternalConfig)
+  function ModifiesInternalConfig(config: InternalConfig): set<object>
+  predicate EncryptStructureEnsuresPublicly(input: EncryptStructureInput , output: Result<EncryptStructureOutput, Error>)
+  // The private method to be refined by the library developer
 
 
- method EncryptStructure ( config: InternalConfig , input: EncryptStructureInput )
- returns (output: Result<EncryptStructureOutput, Error>)
- requires
- && ValidInternalConfig?(config)
- && input.cmm.ValidState()
- modifies ModifiesInternalConfig(config) ,
- input.cmm.Modifies
- // Dafny will skip type parameters when generating a default decreases clause.
- decreases ModifiesInternalConfig(config) ,
- input.cmm.Modifies
- ensures
- && ValidInternalConfig?(config)
- ensures EncryptStructureEnsuresPublicly(input, output)
+  method EncryptStructure ( config: InternalConfig , input: EncryptStructureInput )
+    returns (output: Result<EncryptStructureOutput, Error>)
+    requires
+      && ValidInternalConfig?(config)
+      && input.cmm.ValidState()
+    modifies ModifiesInternalConfig(config) ,
+             input.cmm.Modifies
+    // Dafny will skip type parameters when generating a default decreases clause.
+    decreases ModifiesInternalConfig(config) ,
+              input.cmm.Modifies
+    ensures
+      && ValidInternalConfig?(config)
+    ensures EncryptStructureEnsuresPublicly(input, output)
 
 
- predicate DecryptStructureEnsuresPublicly(input: DecryptStructureInput , output: Result<DecryptStructureOutput, Error>)
- // The private method to be refined by the library developer
+  predicate DecryptStructureEnsuresPublicly(input: DecryptStructureInput , output: Result<DecryptStructureOutput, Error>)
+  // The private method to be refined by the library developer
 
 
- method DecryptStructure ( config: InternalConfig , input: DecryptStructureInput )
- returns (output: Result<DecryptStructureOutput, Error>)
- requires
- && ValidInternalConfig?(config)
- && input.cmm.ValidState()
- modifies ModifiesInternalConfig(config) ,
- input.cmm.Modifies
- // Dafny will skip type parameters when generating a default decreases clause.
- decreases ModifiesInternalConfig(config) ,
- input.cmm.Modifies
- ensures
- && ValidInternalConfig?(config)
- ensures DecryptStructureEnsuresPublicly(input, output)
+  method DecryptStructure ( config: InternalConfig , input: DecryptStructureInput )
+    returns (output: Result<DecryptStructureOutput, Error>)
+    requires
+      && ValidInternalConfig?(config)
+      && input.cmm.ValidState()
+    modifies ModifiesInternalConfig(config) ,
+             input.cmm.Modifies
+    // Dafny will skip type parameters when generating a default decreases clause.
+    decreases ModifiesInternalConfig(config) ,
+              input.cmm.Modifies
+    ensures
+      && ValidInternalConfig?(config)
+    ensures DecryptStructureEnsuresPublicly(input, output)
 }
